t/sum-to-n-recursive.dfy
@@ -1,0 +1,22 @@
+method Verify(n : int) returns (r : int)
+  requires n >= 0
+  ensures  r == n*(n + 1) / 2
+{
+  if (n == 0) {
+    r := n;
+  }
+  if (n > 0) {
+    var s : int;
+    s := Verify(n - 1);
+    r := n + s;
+  }
+}
+
+method Main()
+  returns (r: int)
+  requires true
+  ensures  true
+{
+  assert(Verify(0)  == 0);
+  assert(Verify(3) == 6);
+}
